## Question 1
***
Suppose $a_{1}, a_{2}, a_{3}, \dots$ 
	is a sequence defined as follows:
		$a_{1}=1, \quad a_{2}=3$ 
		$a_{k} = a_{k+2}+2a_{k-1}$ for each integer $k \geq 3$

Prove that $a_{n}$ is odd for every integer $n\geq 1$

1. **Anchor**
Show that property is true for $n=1$ and $n=2$ 
	$a_{1}=1$ and $a_{1}=3$ 
		both $1$ and $3$ are odd

Thus the property is *tme* for $n=1$ and $n=2$

2. **Induction step**
If, for any integer $k>2$
	the property is true for all integers $i$
		such that $1\leq i\leq k$
			*then it is true for $k$* 

*Hint:* Since $a_{k}=a_{k-2}+2a_{k-1}$
	$a_{k}$ is sum of an odd and even integer
		so, $a_{k}$ is odd 

3. **Inductive hypothesis**
Let $k<2$ be an integer,
	and suppose $a_{i}$ 
		is odd
			for all integers $i$ 
				such that $1\leq i\leq k$ 
					is $a_{k}$ odd?
						if so, the statement has been proved.

We know that $a_{k} = a_{k-2}+2a_{k-1}$ 
	by the definition of the sequence

$k-2$ is less than $k$ and is greater than or equal to $1$
	because $k>2$

By inductive hypothesis,
	$a_{k-2}$ is odd

Every term of the sequence is an integer
	(being a sum of product of integers)

$2a_{k-1}$ is even by the definition of even
	(has a $2$ as a factor)

$a_{k}$ is odd 
	because it is the sum of an odd integer 
		and an even integer
			(Needed to be shown)

## Question 2
***
Suppose $b_{1}, b_{2}, b_{3}, \dots$ is a sequence defined as follows:
	$b_{1}=4, \quad b_{2}=12$
	$b_{k}=b_{k-2}+b_{k-1}$ for each integer $k\geq 3$ 

Prove that $b_{n}$ is divisible by $4$ for every integer $n\geq 1$
***
Let the property $P(n)$ be the statement :
$$b_{n} \text{ is divisible by } 4 \leftarrow P(n)$$
We will use strong mathematical induction to prove 
	that for every integer $n\geq 1$
		$P(n)$ is true

**Show that for every integer $k\geq 3$**
**if $P(i)$ is true for each integer $i$ with $1\leq i\leq k$**
**then $P(k+1)$ is true :** 

Let $k$ be any integer with $k\geq 3$
	and suppose that 
		$$b_{i} \text{ is divisible by } 4 \text{ for each integer } i \text{ with } 1\leq i\leq k$$
		**Inductive Hypothesis**

We must show that $b_{k+1}$ is divisible by $4$ ($P(k+1)$) 
But since $k\geq 3$ 
	we have $k+1\geq 3$ and $k-1\geq 2$
		and so
			$b_{k+1}=b_{k-1}+b_{k}$

Moreover, $b_{k-1}$ and $b_{k}$ are both divisible by $4$
	by the inductive hypothesis 
		because both $k$ and $k-1$ 
			are less than or equal to $k$
				so, 
$$
\begin{align}
b_{k+1} &= b_{k-1}+b_{k}\\
&= 4r+4s &\text{ for some integers } r \text{ and } s\\
&= 4(r+s)\\
&= 4t &\text{ for some integer } t 
\end{align}
$$
					$b_{k+1}$ is is divisible by $4$
						hence the property is true for $n=k+1$

**Since we have both the basis 
	and the inductive step 
		of the strong mathematical induction, 
			we conclude that the given statement is true**  

## Question 3
***
Let $c_{0}, c_{1}, c_{2}, \dots$ be the sequence 
	defined by specifying 
		$c_{0}=2$
		$c_{1}=2$ 
		$c_{2}=6$
		$c_{k}=3c_{k-3}$ for every integer $k\geq 3$
			and let the property $\mathcal{P}(n)$ be the statement:
				$$\mathcal{P}(n) \rightarrow c_{n} \text{ is even}$$
***
We will use strong mathematical induction
	to prove that for integer $n\geq 1$ 
		$\mathcal{P}(n)$ is true

**Show that for every integer $k\geq 3$
	if $P(i)$ is true for each integer $i$ 
		with $i\leq i\leq k$
			then $P(k+1)$ is true :**

Let $k$ be any integer with $k\geq 3$
	and suppose that 
		$c_{i}$ is even for each $i$ with $1\leq i\leq k$
			(**Inductive Hypothesis**)

We must show that 
	$$\mathcal{P}(n) \rightarrow c_{k+1} \text{ is even}$$
		but since $k\geq 3$ 
			we have $k+1\geq 3$ and $k-2\geq 1$ 
				and so 
					$$c_{k+1}=3c_{k-2}$$
						by definition of the sequence

Moreover, $c_{k-2}$ is even by the inductive hypothesis
	because $k-1$ is less than or equal to $k$

So, 
$$
\begin{align}
c_{k+1} &= 3c_{k-2}\\
&= 3(2r) &\text{ for some integer } r&\\
&= 2(3r)\\
&= 2t &\text{ for some integer } t
\end{align}
$$

By definition of even 
	$c_{k+1}$ is even
Hence the property is true for $n=k+1$

## Divisibility by a prime 
***
Prove that any integer greater than $1$
	is divisible by a prime number

## Proving a property of a sequence with Strong Induction
***
Let $s_{0}, s_{1}, s_{2}, \dots$
	be the sequence defined by 
		specifying that $s_{0}=1, s_{1}=4$ and $s_{k}=6a_{k-1}-5a_{k-2}$ 
			for every integer $k\geq 2$
				and let the property $P(n)$ be the formula
					$$s_{n}=5^{n}-1$$
We will use ==strong mathematical induction== to prove that 
	for every integer $n\geq 0$ 
		$P(n)$ is true.

**Show that $P(0)$ and $P(1)$ are true :** 
	To establish $P(0)$ and $P(1)$ 
		We must show that 
			$$s_{0}=5^{0}-1 \text{ and } s_{1}=5^{1}-1$$
But by the definition of $s_{0}, s_{1}, s_{2}, \dots$ 
	we have $s_{0}=0$ and $s_{1}=4$
Since $5^{0}-1=0$ and $5^{1}-1=4$,
	the values of $s_{0}$ and $s_{1}$ 
		agree with the values given by the formula

**Show that for every integer $k\geq 1$ 
	if $P(i)$ is true for each integer $i$ from $0$ through $k$
		then, $P(k+1)$ is also true**

Let $k$ be any integer with $k\geq 1$ and suppose that 
	$s_{i}=5^{i}-1$ for each integer $i$ with $0\leq i\leq k$ (**inductive hypothesis**) 

We must show that 
	$$P(k+1)\rightarrow s_{k-1}=5^{k+1}-1$$
but since $k\geq 1$ 
	we have that $k+1\geq 2$
		and so
$$
\begin{align}
s_{k+1} &= 6s_{k}-5s_{k-1} & &\text{ by definition of sequence}\\
&= 6(5^{k}-1)-5(5^{k-1}-1) & &\text{ by definition hypothesis}\\
&= 8\cdot 5^{k} - 6 - 5^{k} + 5 & &\text{ by multiplying out and applying} \\
& & & \quad\text{a law of exponents}\\
&= (6-1)5^{k} - 1 & &\text{ by factoring out 6 and arithmetic}\\
&= 5 \cdot 5^{k}-1 & &\text{ arithmetic}\\
&= 5^{k+1}-1 & &\text{ applying law of exponents}
\end{align}
$$

## Quotient-Remainder Theorem (Existence)
***
Given any integer $n$ and any positive integer $d$, 
	there exists integers $q$ and $r$ such that 
		$$n = dq + r \quad \textbf{ and } \quad 0\leq r\leq d$$

**Proof :** Let $S$ be the set of all nonnegative integers of the form
	$$n-dk,$$
			where $k$ is an integer.

This set has at least one element 
	{ *for if $n$ is nonnegative, then 
	$$n-0 \cdot d = n\geq 0$$
	and so $n-0 \cdot d$ is in $S$. And if $n$ is negative, then 
$$
\begin{align}
n-nd=n &\underbrace{(1-d)}\geq 0\\
&\tiny{{\leq \ 0\text{ since } d \text{ is a positive integer}}}&
\end{align}
$$
	and so $n-nd$ is in $S$*}

It follows by the well-ordering principle for the integer that $S$ contains a least element $r$
Then, for some specific integer value of $k$, say $q$
$$n-dq=r$$
	(*because every integer in $S$ can be written in this form*) 

Adding $dq$ to both sides gives 
$$n=dq + r$$
Furthermore, $r<d$ (*For suppose $v\geq d$. Then*)
$$n-d(q+1)=n-dq-d=r-d\geq 0$$
and so $n-d(q+1)$ 
	would be a nonnegative integer in $S$ 
		that would be smaller than $r$
But $r$ is the smallest integer in $S$ 
This contradiction shows that the supposition $r\geq d$
	must be false.
this preceding arguments prove that there exists integers $r$ and $q$ for which 
$$n=dq+r \textbf{ and } 0\leq r\leq d$$

**Strictly decreasing sequence of nonnegative integers is finite**





