**Example 2.1**
If $P=X^{2}+1$, then $P=(X-i)(X+i)$. The zeroes/roots are $z_{1}=i$ and $z_{2}=-i$, and both have multiplicity 1 .

  

If $P=\left(X^{2}+1\right)^{2}=X^{4}+2 X^{2}+1$, then $P=(X-i)^{2}(X+i)^{2}$. The roots are $z_{1}=i$ and $z_{2}=-i$, and both have multiplicity 2 .

  

If $P=X(X+1)(X-i)^{2}$, then the roots are $z_{1}=0, z_{2}=-1$, and $z_{3}=i$. The multiplicities are $m_{1}=m_{2}=1$ and $m_{3}=2$, and the sum of the multiplicities is $1+1+2=4$, the degree of the polynomial.

A rational function is a quotient of two polynomial functions:

  

$$

f(z)=\frac{P(z)}{Q(z)} .

$$

  

If $z_{0}$ is a zero of $Q$ of multiplicity $m_{Q}$ and a zero of $P$ of multiplicity $m_{P}$, then $P(z)=\left(z-z_{0}\right)^{m_{P}} P_{1}(z), Q(z)=\left(z-z_{0}\right)^{m_{Q}} Q_{1}(z)$, and

  

$$

f(z)=\frac{\left(z-z_{0}\right)^{m_{P}} P_{1}(z)}{\left(z-z_{0}\right)^{m_{Q}} Q_{1}(z)}=\left(z-z_{0}\right)^{m_{P}-m_{Q}} \frac{P_{1}(z)}{Q_{1}(z)} .

$$

  

Since $P_{1}\left(z_{0}\right) \neq 0 \neq Q_{1}\left(z_{0}\right)$, it follows that, after simplifying the common powers of $z-z_{0}$ from $P$ and $Q$, the function $f$ can be defined at $z_{0}$ if and only if $m_{P} \geqslant m_{Q}$.

  

Let $f(z)=\frac{P(z)}{Q(z)}$ be a rational function, such that $P$ and $Q$ do not have any common zeroes - we will call such a rational function reduced and unless explicitly specified otherwise, all the rational functions we will consider are reduced. A zero $z_{0}$ of $P$ is called a zero of $f$, and the multiplicity of $z_{0}$ as a zero of $f$ is the multiplicity of $z_{0}$ as a zero of $P$. A zero $z_{0}$ of $Q$ is called a pole of $f$, and the multiplicity of $z_{0}$ as a zero of $Q$ is called the order of the pole $z_{0}$ of $f$. The domain of $f=P / Q$ is $\mathbb{C}$ minus the set of all its poles - the entire plane with a finite number reduced rational function zero pole order of a pole of points removed.

  

**EXAMPLE 2.2.**
Let

  

$$

f(z)=\frac{z(z+1)(z-i)^{2}}{(z+i)^{2}(z-1)}

$$

  

The zeroes of $f$ are $0,-1$, and $i$, with multiplicities 1,1 , and 2 , respectively. The poles of $f$ are $-i$ and 1 , with orders 2 and 1 , respectively. The domain of $f$ is $\mathbb{C} \backslash\{1,-i\}$.

  
**EXAMPLE 2.3**
Let $f_{1}(z)=z+a, f_{2}(z)=b z+c$, and $f_{3}(z)=1 / z$. Then

  

$$

\begin{aligned}

\left(f_{2} \circ f_{3} \circ f_{1}\right)(z) & =\left(f_{2} \circ f_{3}\right)(z+a)=f_{2}\left(\frac{1}{z+a}\right)=\frac{b}{z+a}+c \\

& =\frac{c z+(a c+b)}{z+a} \\

\left(f_{1} \circ f_{3} \circ f_{2}\right)(z) & =\left(f_{1} \circ f_{3}\right)(b z+c)=f_{1}\left(\frac{1}{b z+c}\right)=\frac{1}{b z+c}+a \\

& =\frac{(a b) z+(a c+1)}{b z+c} .

\end{aligned}

$$

  

In both cases the end result is a rational function, with polynomials of degree 1 as numerators and denominators.

**EXAMPLE 2.4**
The unique Möbius transformation that sends the triple $(-1,0,1)$ to $(0,1, i)$ is the solution of the equation

  

$$

\begin{aligned}

& \frac{f(z)-1}{f(z)-i}: \frac{0-1}{0-i}=\frac{z-0}{z-1}: \frac{-1-0}{-1-1} \Longleftrightarrow \\

& \frac{f(z)-1}{f(z)-i} \cdot i=\frac{z}{z-1} \cdot 2 \Longleftrightarrow f(z)=\frac{-z-1}{(2 i+1) z-1} .

\end{aligned}

$$

  

**ExAMPLE 2.5**
To find the unique Möbius transformation that sends the triple $(0,1, i)$ to $(i, 1, \infty)$, we take advantage of the presence of $\infty$ in the second triple and use the equality of cross-ratios

  

$$

(f(z), \infty ; i, 1)=(z, i ; 0,1)

$$

  

Then $f(z)$ is the solution of the equation

  

$$

\begin{aligned}

& \frac{f(z)-i}{f(z)-1}: \frac{\infty-i}{\infty-1}=\frac{z-0}{z-1}: \frac{i-0}{i-1} \Longleftrightarrow \\

& \frac{f(z)-i}{f(z)-1}=\frac{(i-1) z}{i(z-1)} \Longleftrightarrow f(z)=\frac{-i z+1}{z-i}

\end{aligned}

$$

  

To understand the geometric transformations that build $f$, we use

  

$$

\begin{aligned}

f(z) & =\frac{-i z+1}{z-i}=(-i) \frac{z+i}{z-i}=(-i)\left(1+\frac{2 i}{z-i}\right)=-i+\frac{2}{z-i} \\

& =2\left(\frac{1}{z-i}-i\right)+i .

\end{aligned}

$$

  

Therefore $f$ is the translation by $-i$, followed by an inversion, and then by a homothety of ratio 2 with center $i$.

  

**EXAMPLE 2.6**
Let $z=1$ and $n=5$; we want to find the complex numbers $\zeta$ such that $\zeta^{5}=1$. Since de Moivre's formula (1.4) provides a nice way of computing powers of complex numbers in trigonometric form, we will work with trigonometric forms of complex numbers. We therefore look for $\zeta=\rho(\cos \alpha+i \sin \alpha)$ such that

  

$$

1=\cos 0+i \sin 0=(\rho(\cos \alpha+i \sin \alpha))^{5}=\rho^{5}(\cos (5 \alpha)+i \sin (5 \alpha)) .

$$

  

Equating the moduli and the argument sets we obtain

  

$$

\rho^{5}=1 \quad \text { and } \quad 5 \alpha=2 k \pi, \text { for some } k \in \mathbb{Z},

$$

  

from which we conclude that

  

$$

\rho=1 \quad \text { and } \quad \alpha=\frac{2 k \pi}{5}, \text { for some } k \in \mathbb{Z} .

$$

  

The modulus is therefore equal to 1 for all solutions of $\zeta^{5}=1$. Different values $k_{1}$ and $k_{2}$ of $k$ will result in the same value for $\zeta$ if and only if the corresponding values of $\alpha$ differ by an integer multiple of $2 \pi$, and that is the case if and only if $k_{1}$ and $k_{2}$ differ by a multiple of 5 . As a consequence, there are exactly five different values for $\zeta$, corresponding to $k=0,1,2,3,4$. The solutions of $\zeta^{5}=1$ are therefore given by

  

$$

\begin{aligned}

& \zeta_{0}=\cos 0+i \sin 0=1 \\

& \zeta_{1}=\cos \frac{2 \pi}{5}+i \sin \frac{2 \pi}{5}:=\omega \\

& \zeta_{2}=\cos \frac{4 \pi}{5}+i \sin \frac{4 \pi}{5}=\omega^{2} \\

& \zeta_{3}=\cos \frac{6 \pi}{5}+i \sin \frac{6 \pi}{5}=\omega^{3} \\

& \zeta_{4}=\cos \frac{8 \pi}{5}+i \sin \frac{8 \pi}{5}=\omega^{4}

\end{aligned}

$$

  

All five are on the unit circle and the angles between consecutive ones are all equal to $\frac{2 \pi}{5}$; therefore $\zeta_{0}=1, \zeta_{1}=\omega, \zeta_{2}=\omega^{2}, \zeta_{3}=\omega^{3}$ and $\zeta_{4}=\omega^{4}$ are the vertices of a regular pentagon.

**EXAMPLE 2.7**
The $4^{\text {th }}$-roots of unity are

$$
\begin{aligned}
1 & =\cos \left(0 \cdot \frac{2 \pi}{4}\right)+i \sin \left(0 \cdot \frac{2 \pi}{4}\right)=\cos 0+i \sin 0 \\
\omega & =\cos \left(1 \cdot \frac{2 \pi}{4}\right)+i \sin \left(1 \cdot \frac{2 \pi}{4}\right)=\cos \frac{\pi}{2}+i \sin \frac{\pi}{2}=i \\
\omega^{2} & =\cos \left(2 \cdot \frac{2 \pi}{4}\right)+i \sin \left(2 \cdot \frac{2 \pi}{4}\right)=\cos \pi+i \sin \pi=-1 \\
\omega^{3} & =\cos \left(3 \cdot \frac{2 \pi}{4}\right)+i \sin \left(3 \cdot \frac{2 \pi}{4}\right)=\cos \frac{3 \pi}{2}+i \sin \frac{3 \pi}{2}=-i
\end{aligned}
$$

and they are the roots of

$$
X^{4}-1=\left(X^{2}-1\right)\left(X^{2}+1\right)=(X-1)(X+1)(X-i)(X+i) .
$$

**EXAMPLE 2.8**
We can now find the roots of $X^{4}+1$; those are the solutions of $\zeta^{4}=-1=\cos \pi+i \sin \pi$; we will work with the trigonometric form and look for $\zeta=\rho(\cos \alpha+i \sin \alpha)$ such that

$$
\cos \pi+i \sin \pi=(\rho(\cos \alpha+i \sin \alpha))^{4}=\rho^{4}(\cos (4 \alpha)+i \sin (4 \alpha)) .
$$

Equating the moduli and the argument sets we obtain

$$
\rho^{4}=1 \quad \text { and } \quad 4 \alpha=\pi+2 k \pi, \text { for some } k \in \mathbb{Z},
$$

from which we conclude that

$$
\rho=1 \quad \text { and } \quad \alpha=\frac{\pi}{4}+\frac{2 k \pi}{4}, \text { for some } k \in \mathbb{Z} .
$$

The values of $\alpha$ for $k=0,1,2,3,4$ are given by

$$
\frac{\pi}{4}, \frac{\pi}{4}+\frac{\pi}{2}, \frac{\pi}{4}+\pi, \frac{\pi}{4}+\frac{3 \pi}{2}, \frac{\pi}{4}+2 \pi
$$

and we note that, in general, for every integer $k$, the values for $k$ and for $k+4$ differ by $2 \pi$, hence they correspond to the same argument set, hence to the same complex number $\zeta$. There are exactly 4 complex numbers $\zeta$ such that $\zeta^{4}=-1$; those four numbers have the same modulus, 1 , and their argument sets are spaced in increments of $\pi / 2$. Let

$$
\zeta_{0}=\cos \left(\frac{\pi}{4}\right)+i \sin \left(\frac{\pi}{4}\right)
$$

be the first of those solutions and

$$
\omega=\cos \left(\frac{\pi}{2}\right)+i \sin \left(\frac{\pi}{2}\right)=i .
$$

Then the four solutions of $\zeta^{4}=-1$ are

$$
\zeta_{0}, \zeta_{0} \omega, \zeta_{0} \omega^{2}, \zeta_{0} \omega^{3}
$$

they correspond to $\zeta_{0}$ and the images of successive counterclockwise rotations of angle $\frac{\pi}{2}$ about the origin, until, after four such rotations, we get back to $\zeta_{0}$. Therefore the solutions of $\zeta^{4}=-1$ are the vertices of a square centered at the origin. That square is obtained from the square corresponding to $4^{\text {th }}$-roots of unity, rotated counterclockwise by an angle $\frac{\pi}{4}=\frac{1}{4} \operatorname{Arg}(-1)$.

**EXAMPLE 2.9**
Let $z=1+i$; we want to find the complex numbers $\zeta$ such that $\zeta^{6}=z$. We will work with trigonometric forms of complex numbers. Then

$$
z=1+i=\sqrt{2}\left(\cos \frac{\pi}{4}+i \sin \frac{\pi}{4}\right)
$$

and we look for $\zeta=\rho(\cos \alpha+i \sin \alpha)$ such that

$$
\sqrt{2}\left(\cos \frac{\pi}{4}+i \sin \frac{\pi}{4}\right)=(\rho(\cos \alpha+i \sin \alpha))^{6}=\rho^{6}(\cos (6 \alpha)+i \sin (6 \alpha)) .
$$

Equating the moduli and the argument sets we obtain

$$
\rho^{6}=\sqrt{2} \quad \text { and } \quad 6 \alpha=\frac{\pi}{4}+2 k \pi, \text { for some } k \in \mathbb{Z},
$$

from which we conclude that

$$
\rho=(\sqrt{2})^{1 / 6} \quad \text { and } \quad \alpha=\frac{\pi}{24}+\frac{2 k \pi}{6}, \text { for some } k \in \mathbb{Z} .
$$

The values of $\alpha$ for $k=0,1,2,3,4,5,6$ are given by

$$
\frac{\pi}{24}, \frac{\pi}{24}+\frac{\pi}{3}, \frac{\pi}{24}+\frac{2 \pi}{3}, \frac{\pi}{24}+\pi, \frac{\pi}{24}+\frac{4 \pi}{3}, \frac{\pi}{24}+\frac{5 \pi}{3}, \frac{\pi}{24}+2 \pi
$$

and we note that, in general, for every integer $k$, the values for $k$ and for $k+6$ differ by $2 \pi$, hence they correspond to the same argument set, hence to the same complex number $\zeta$. There are exactly 6 complex numbers $\zeta$ such that $\zeta^{6}=1+i$; those six numbers have the same modulus, $(\sqrt{2})^{1 / 6}$, and their argument sets are spaced in increments of $\pi / 3$. Let

$$
\zeta_{0}=(\sqrt{2})^{1 / 6}\left(\cos \left(\frac{\pi}{24}\right)+i \sin \left(\frac{\pi}{24}\right)\right)
$$

be the first of those solutions and

$$
\omega=\cos \left(\frac{\pi}{3}\right)+i \sin \left(\frac{\pi}{3}\right)
$$

Then the six solutions of $\zeta^{6}=1+i$ are

$$
\zeta_{0}, \zeta_{0} \omega, \zeta_{0} \omega^{2}, \zeta_{0} \omega^{3}, \zeta_{0} \omega^{4} \text {, and } \zeta_{0} \omega^{5}
$$

they correspond to $\zeta_{0}$ and the images of successive counterclockwise rotations of angle $\frac{\pi}{3}$ about the origin, until, after six such rotations, we get back to $\zeta_{0}$. Therefore the solutions of $\zeta^{6}=1+i$ are the vertices of a regular hexagon centered at the origin. That hexagon is obtained from the regular hexagon corresponding to $6^{\text {th }}$-roots of unity, rotated counterclockwise by an angle $\frac{\pi}{24}=\frac{1}{6} \operatorname{Arg}(1+i)$ and rescaled by a factor of $(\sqrt{2})^{1 / 6}=|1+i|^{1 / 6}$.

**EXAMPLE 2.10**
For $w=z^{2}$ we have

$$
u+i v=(x+i y)^{2}=x^{2}-y^{2}+i(2 x y),
$$

hence $u(x, y)=x^{2}+y^{2}$ and $v(x, y)=2 x y$.

For $w=\bar{z}$ we have

$$
u+i v=\overline{x+i y}=x-i y,
$$

hence $u(x, y)=x$ and $v(x, y)=-y$.

For $w=|z|$ we have

$$
u+i v=|x+i y|=\sqrt{x^{2}+y^{2}},
$$

hence $u(x, y)=\sqrt{x^{2}+y^{2}}$ and $v(x, y)=0$.