Question 3: Show that for a fixed point iteration procedure pn+1=g(pn)pn+1=g(pn)p_{n+1}=g(p_n) with |g′(x)|≤K<1,|pn−p|≤Kn1−K|p1−p0|g ′(x)|≤K<1,|pn−p|≤Kn1−K|p1−p0|g'(x)|\leq K < 1, |p_n-p| \leq \cfrac{K^n}{1-K} |p_1-p_0 Proof: Given a fixed point iteration procedure defined by pn+1=g(pn)pn+1=g(pn) p_{n+1} = g(p_n) we aim to demonstrate that if |g′(x)|≤K<1|g′(x)|≤K<1 |g'(x)| \leq K < 1 for all ( x ), then |pn−p|≤Kn1−K|p1−p0||pn−p|≤Kn1−K|p1−p0| |p_n-p| \leq \frac{K^n}{1-K} |p_1-p_0| for all ( n ). We will employ Mathematical Induction. Consider the error iteration formula for fixed point iteration: en+1=|pn+1−p|en+1=|pn+1−p| e_{n+1} = |p_{n+1}-p| en=|pn−p|en=|pn−p| e_n = |p_n - p| By invoking the Mean Value Theorem, which states: If a function ( f ) is continuous on the closed interval ([a, b]) and differentiable on the open interval ((a, b)), then there exists at least one number ( c ) in the open interval ((a, b)) such that: f′(c)=f(b)−f(a)b−af ′(c)=f(b)−f(a)b−a f'(c) = \frac{f(b)-f(a)}{b-a} there exists a number ( c ) between ( p ) and ( p_n ) such that: g′(c)=g(pn)−g(p)pn−pg′(c)=g(pn)−g(p)pn−p g'(c) = \frac{g(p_n)-g(p)}{p_n-p} Rearranging, we obtain: g(pn)−g(p)=g ′(c)(pn−p)g(pn)−g(p)=g′(c)(pn−p) g(p_n)-g(p) = g'(c)(p_n-p) Given ( p_{n+1} = g(p_n) ) and ( p = g(p) ) (since ( p ) is a fixed point), substituting into the above equation yields: pn+1−p=g′(c)(pn−p)pn+1−p=g′(c)(pn−p) p_{n+1}-p = g'(c)(p_n-p) Taking the absolute value, we get: |pn+1−p|=|g ′(c)|×|pn−p||pn+1−p|=|g′(c)|×|pn−p| |p_{n+1}-p| = |g'(c)| \times |p_n-p| or equivalently, en+1=|g ′(c)|×enen+1=|g′(c)|×en e_{n+1} = |g'(c)| \times e_n Given the condition ( |g'(x)| \leq K ), it follows that: en+1≤K×enen+1≤K×en e_{n+1} \leq K \times e_n Base Case: For ( n = 1 ): e2≤K×e1e2≤K×e1 e_2 \leq K \times e_1 This is validated by the previous equation. Inductive Step: Assuming the inequality holds for ( n = k ): ek+1≤Kk1−K×e1ek+1≤Kk1−K×e1 e_{k+1} \leq \frac{K^k}{1-K} \times e_1 From our derived inequality, we infer: ek+2≤K×ek+1ek+2≤K×ek+1 e_{k+2} \leq K \times e_{k+1} Substituting our inductive assumption into this gives: ek+2≤K×Kk1−K×e1ek+2≤K×Kk1−K×e1 e_{k+2} \leq K \times \frac{K^k}{1-K} \times e_1 or ek+2≤Kk+11−K×e1ek+2≤Kk+11−K×e1 e_{k+2} \leq \frac{K^{k+1}}{1-K} \times e_1 By induction, this inequality stands for all ( n ). Lastly, given ( e_1 = |p_1 - p_0| ), we deduce: en+1≤Kn1−K×|p1−p0|en+1≤Kn1−K×|p1−p0| e_{n+1} \leq \frac{K^n}{1-K} \times |p_1-p_0| This completes the proof of the given inequality.