| $$\neg{x\neg{y}+\neg{x}z}$$                              | rules             |
| -------------------------------------------------------- | ----------------- |
| $$(\neg{(x\neg{y}))}\cdot (\neg{(\neg{x}z)}$$            | DeMorgan's Law    |
| $$(\neg{x}+\neg{\neg{y})}\cdot (\neg{\neg{x}}+\neg{z})$$ | DeMorgan's Law    |
| $$(\neg{x}+y)\cdot (x+\neg{z})$$                         | Double Complement |
$$\therefore \overline{(x\overline{y})(x+\overline{z})} = (\overline{x}+y)\cdot (x+\overline{z}) $$

| Expression                                       | Rule used         |
| ------------------------------------------------ | ----------------- |
| $$(\neg{x}+\neg{y})\cdot (\neg{(\neg{(x+y)})})$$ | DeMorgan's Law    |
| $$(\neg{x}+\neg{y})\cdot (x+y)$$                 | Double Complement |
| $$\neg{x}x+\neg{x}y+\neg{y}x+\neg{y}y$$          | Algebra           |
| $$(\neg{x}y)+(\neg{y}x)+0+0$$                    | Complement Law's  |
| $$(\neg{x}y)+(\neg{y}x)$$                        | $\therefore$ DNF is attained.                   |


