Direct Proof

An Implication $p \rightarrow q$ can be proved 
- By showing that if $p$ is true
	- the $q$ is also true
*Assume the hypothesis of implication is true*

Indirect Proof

An implication $p\rightarrow q$  is equivalent
- to its contrapositive $\neg q \rightarrow \neg p$ 
	- Therefore, 
		- we can prove $p\rightarrow q$ 
			- by showing that whenever $q$ is false 
				- $p$ is also false
*Assume that the conclusion of the implication is false*
- *Then show hypothesis must also be false.*
	- *use rules of inference and known theorems*
(Showing contrapositive is true) 
- (equivalent to showing implication is also true)

Proof by Contradiction

*Assume theorem is false*
- *Then show that this contradicts with the assumption*
	- *Therefore the theorem has to be true*

Proof by Cases
$n \times (n+1)$ 
$n \times m$ where $m = (n+1)$

case 1: n is odd : m is even 
case 2: n is even : m is even