
# Question 9
A car slows down from $28\left[ \frac{m}{s} \right]$ to rest in a distance of $88[m]$
What was its acceleration, assumed constant?
# Question 10
Determine the stopping distances for a car going at a constant initial speed of $95\left[ \frac{m}{s^2} \right]$ and human reaction of $0.40\left[ s \right]$ for a) and b) below, 
***
This is a two part problem:
1. How far does the car go before the reaction happens?
2. How far does it take to stop after reaction causes braking?

For 1, reaction distance can be found from $\bar{s}$ and  $\Delta t$ :
- Givens:
	- $\bar{s} = 95\left[ \cfrac{km}{h} \right]\cdot \left( \cfrac{100[m]}{1[km]} \right) \cdot \left( \cfrac{1[h]}{3600[s]} \right)=26.39\left[ \frac{m}{s} \right]$
	- $\Delta t=0.40[s]$ 
- Equation, solve for $D$
	- $\bar{S}=\cfrac{D}{\Delta t}$
	- $D = \bar{s}\Delta t=\left( 26.39\left[ \frac{m}{s} \right] \right)\left( 0.40[s] \right)=10.56[m]$

For part 2, the starting position is $D$:
$$x_{0}=D=10.56[m]$$
- Givens:
	- $v=0.0\left[ \frac{m}{s} \right]$ 
	- $v_{0}=\bar{s}=26.39\left[ \frac{m}{s} \right]$
	- $$a =\begin{cases}
&-3.0\left[ \frac{m}{s^2} \right] ;(a) \\
& -6.0\left[ \frac{m}{s^2} \right] ;(b)\\
\end{cases}$$
	- $x_{0} = D = 10.56[m]$

We want $x$,
so we solve $v^2=v_{0}^2+2a(x-x_{0})$
$$
\begin{align}
v^2-v_{0}^2&=2a(x-x_{0})\\
\cfrac{v^2-v_{0}^2}{2a}&=x-x_{0} \\
x&=x_{0}+\cfrac{v^2-v_{0}^2}{2a}
\end{align}
$$

## a) So when we have acceleration of $a = -3.0\left[ \cfrac{m}{s^2} \right]$
$$
\begin{align}
x&=x_{0}+\cfrac{v^2-v_{0}^2}{2a} \\
&=126.6[m] \\
&\approx 130[m]
\end{align}
$$
## b) an acceleration of $a = -6.0\left[ \cfrac{m}{s^2} \right]$

$$
\begin{align}
x & =x_{0}+\cfrac{v^2-v_{0}^2}{2a} \\
 & =68.60[m] \\
 & \approx 69[m]
\end{align}
$$







# Question 11

A stone is thrown vertically upward with a speed of $24.0\left[ \frac{m}{s} \right]$ 
## a)
How fast is it moving when it is at a height of $13[m]$ 
We can use the kinematic equation: $$ v^2 = v_0^2 - 2g(h - h_0) $$ where we are given:
Initial velocity: $v_{0}=24.0\left[ \cfrac{m}{s} \right]$
Final height: $h=13.0 \left[ m \right]$
$h_{0}=0[m]$
Acceleration due to gravity : $g = 9.8 \left[ \cfrac{m}{s^2} \right]$
and where,
-
***
We will use the following kinematic equations to solve the problem:
$$
\begin{align}
& 1. \ v^2=v_{0}^2-2g(h-h_{0})(\text{to find the velocity at height}) \  \\
& 2. \ h=v_{0}t-\frac{1}{2}gt^{2} \ (\text{to find time to reach height }\ h) 
\end{align}
$$

Substituting these values: $$ v^2 = (24.0)^2 - 2(9.8)(13) $$ $$ v^2 = 576 - 254.8 $$ $$ v^2 = 321.2 $$ $$ v = \sqrt{321.2} \approx 17.92 \, \text{m/s} $$ So, the stone is moving at approximately $17.9 \left[ \cfrac{m}{s} \right]$when it reaches a height of 13 meters.
## b)
How much time is required to reach this height?
We use the equation: $$ h = v_0 t - \frac{1}{2} g t^2 $$ Substituting the known values: $$ 13 = 24t - \frac{1}{2} (9.8) t^2 $$ $$ 13 = 24t - 4.9t^2 $$ Rearranging the equation: $$ 4.9t^2 - 24t + 13 = 0 $$ This is a quadratic equation. Using the quadratic formula: $$ t = \frac{-(-24) \pm \sqrt{(-24)^2 - 4(4.9)(13)}}{2(4.9)} $$ $$ t = \frac{24 \pm \sqrt{576 - 254.8}}{9.8} $$ $$ t = \frac{24 \pm \sqrt{321.2}}{9.8} $$ $$ t = \frac{24 \pm 17.92}{9.8} $$ This gives two possible times: $$ t_1 = \frac{24 + 17.92}{9.8} = \frac{41.92}{9.8} \approx 4.28 \, \text{seconds} $$ $$ t_2 = \frac{24 - 17.92}{9.8} = \frac{6.08}{9.8} \approx 0.620 \, \text{seconds} $$
## c)
why are there two answers to b)?

There are two answers to part b) because the stone passes through the height of 13 meters twice: once on the way up and once on the way down. The first time $( t_2 )$ corresponds to the moment when the stone is moving upward, and the second time $( t_1 )$ corresponds to when the stone is falling back down after reaching its maximum height.

# 12 
The acceleration due to gravity on the Moon is about one-sixth of what it is on Earth. If an object is thrown vertically upward on the moon. how many times higher will it go than it would on Earth, assuming the same initial velocity?

## Solution:
Given:
$v_{0}$
$v$
$a$

and we want $y-y_{0}$
***
Lets use the equation $$v^2=v_{0}^2+2a(y-y_{0})$$
- use $\Delta y=y-y_{0}$ and $v=0$ (at peak of trajectory)
- $$0=v_{0}^2+2a\Delta y$$
- solve for $\Delta y$:
	- $$\Delta y=-\cfrac{v_{0^2}}{2a}$$
On Earth:
$$a_{\oplus}=-g$$
- so,
$$\Delta y_{\oplus}=-\cfrac{v_{0}^2}{2(-g)}=\cfrac{v_{0}^2}{2g}$$
On the Moon:
$$a_{\odot}=-\cfrac{g}{6}$$
so, 
$$\Delta y_{\odot}=-\cfrac{v_{0^2}}{2-\left( \frac{g}{6} \right)}=\cfrac{3v_{0}^2}{g}$$

so the ratio of displacement 'on' the Moon to displacement on earth is:
$$
\cfrac{\Delta y_{\odot}}{\Delta y_{\oplus}}=\cfrac{3v_{0}^{2}}{g} \cdot \cfrac{1}{\left( \frac{v_{0}^2}{2g} \right) }=\frac{3v_{0}^2}{g}\cdot
\cfrac{2g}{v_{0}^2}=6
$$
so the object travels $6$ times farther upward "on" the moon than on "on" Earth.