$$
\begin{align}
(Q \mathbf{x})^{*} \, (Q \mathbf{y}) &= \mathbf{x}^{*} \, \mathbf{y}\, Q\, Q^{*}\\
&= \mathbf{x}^{*} \, \mathbf{y} \, I_{n}\\
&= \mathbf{x}^{*} \, \mathbf{y}
\end{align}
$$

$$
\begin{align}
\|\mathbf{x}\| &= \|Q\mathbf{x}\|\\
\| \mathbf{x}\| &= \|Q\,Q^{-1}| \ \|\mathbf{x}\|\\
\text{or} \quad \|\mathbf{x}\| &= |Q\,Q^{*}| \ \|\mathbf{x}\|\\
\|\mathbf{x}\| &=I_{m}\cdot\ \|\mathbf{x}\|\\
\end{align}
$$

$$
\begin{bmatrix}
\left\langle\vec{n_{j}},\vec{n_{k}}\right\rangle
\end{bmatrix}
= 
\begin{bmatrix}
\delta_{jk}
\end{bmatrix}
=
I_{m} 
\quad\quad \text{for}\ 1\leq j,\,k \leq m
$$

$$
\begin{bmatrix}
\vec{n_{1}} \, \vec{n_{1}^{*}} & \cdots & \vec{n_{m}} \, \vec{n_{1}^{*}}\\
\vdots & \ddots & \vdots\\
\vec{n_{1}} \, \vec{n_{m}^{*}} & \cdots & \vec{n_{m}} \, \vec{n_{m}^{*}}\\
\end{bmatrix}
=
$$

$$ 
QQ^{*} 
= 
\begin{bmatrix} 
\vec{n_{1}} & \vec{n_{2}} & \cdots & \vec{n_{m}}
\end{bmatrix}
\,
\begin{bmatrix}
\vec{n_{1}^{*}}\\ 
\vec{n_{2}^{*}}\\ 
\vdots\\ 
\vec{n_{m}^{*}}
\end{bmatrix}
=
$$