To begin, set $a_1=-2$ and $b_1=1.5$. We notice that $$\begin{align*} f(a_1)&=f(-2)=3(-2+1)(-2-1/2)(-2-1)=-\frac{45}{2}<0\\ f(b_1)&=f(1.5)=3(1.5+1)(1.5-1/2)(1.5-1)=3.75>0 \end{align*}$$ So that, we can say that there exists at leas one real $p$ in the interval $(-2,1.5)$ such that $f(p)=0$. Let us consider the midpoint $$p_1=\frac{a_1+b_1}{2}=\frac{-2+1.5}{2}=-0.25$$ We can notice that $$ f(p_1)=f(-0.25)=3(-0.25+1)(-0.25-1/2)(-0.25-1)=2.10938>0 $$ Since $f(p_1)$ and $f(a_1)$ have different sign, a root $p$ of the function is in the interval $(a_1,p_1)$. So that, we set $a_2=a_1=-2$ and $b_2=p_1=-0.25$. For these new extremes, ($a_2,\ b_2$), we have that $$p_2=\frac{a_2+b_2}{2}=\frac{-2-0.25}{2}=-1.125$$ Since $$f(p_2)=f(-1.125)=-1.29492<0$$ and $f(b_2)=f(p_1)=2.10938>0$ have opposite signs, a root of the function is in the interval $(-1.125,-0.25)$. Finally, we set $a_3=p_2$ and $b_3=b_2=-0.25$ for which $$p_3=\frac{a_3+b_3}{2}=\frac{-1.125+(-0.25)}{2}=-0.6875$$
3 

To have a solution accurate within $10^{-2}$, we can use that $$\begin{equation} \frac{b-a}{2^n}<10^{-2} \end{equation}$$ In this case we have that $a=0$ and $b=1$, hence from equation (1) we have that there are required $$ \frac{b-a}{2^n}<10^{-2}\Rightarrow \frac{1}{2^n}<10^{-2}\Rightarrow 2^n>100\Rightarrow n>6$$ at least 7 iterations to have a solution accurate within $10^{-2}$. Now, we can notice that $$\begin{align*} f(0)&=(0)^3 - 7 (0)^2 + 14 (0) - 6=-6<0\\ f(1)&=(1)^3 - 7 (1)^2 + 14 (1) - 6=2>0 \end{align*}$$ Since $f(0)$ and $f(1)$ have opposite signs, we can ensure that in the interval the function $f$ have at least one real root. We need to use 7 iterations to obtain $p_7$. To begin, we set $a_1=a=0$ and $b_1=b=1$. So the midpoint is $$p_1=\frac{a_1+b_1}{2}=\frac{0+1}{2}=\frac{1}{2}$$ Since $f(1/2)=-\frac{5}{8}<0$ and $f(1)=2>0$ have opposite signs, a root of the function is located in the interval $(1/2,1)$. So that, for the second iteration we set $a_2=p_1=1/2$ and $b_2=b_1=1$. **This procedure is carried out until finding $p_7$ in the $7^{th}$ iteration**. For $a_2=1/2$ and $b_2=1$, $$p_2=\frac{a_2+b_2}{2}=\frac{1/2+1}{2}=\frac{3}{4}\Rightarrow f(p_2)=f(3/4)=63/64>0$$ Since $f(p_2)>0$ and $f(a_2)=f(1/2)<0$ we set $a_3=a_2=1/2$ and $b_3=p_2=3/4$. In this case, $$p_3=\frac{a_3+b_3}{2}=\frac{1/2+3/4}{2}=5/8\Rightarrow f(p_3)=f(5/8)=133/512>0$$ Since $f(p_3)>0$ and $f(a_3)=f(1/2)<0$ we set $a_4=a_3=1/2$ and $b_4=p_3=5/8$. In this case, $$p_4=\frac{a_4+b_4}{2}=\frac{1/2+5/8}{2}=9/16\Rightarrow f(p_4)=f(9/16)=-663/4096<0$$