$$
\begin{align}
\overrightarrow{u} &= \langle \, -1, 2, 3 \, \rangle\\ \overrightarrow{v} &= \langle \, 2, -3, 5 \, \rangle\\ \overrightarrow{w} &= \langle \, 3, 5, -7 \, \rangle\\
\end{align}
$$

# Carry out the the indicated operations between the vectors indicated.

- $-\overrightarrow{u}$
- $\overrightarrow{u} + \overrightarrow{w} - (\, 2\overrightarrow{v} + \overrightarrow{u}\,)$
- $\overrightarrow{u} \, \cdot \, \overrightarrow{v}$

Samir Banjara
Due:  Feb 8th 11:59pm

## Question 1
- $-\overrightarrow{u}$
$$
\begin{align}
-\overrightarrow{u} &= (-1)\cdot \overrightarrow{u}\\
&=\langle \,(-1)\cdot (-1),\ 2\cdot (-1) ,\ 3\cdot (-1) \,\rangle\\ 
&= \langle \, 1, -2, -3 \, \rangle\\
\end{align}
$$

## Question 2
- $\overrightarrow{u} + \overrightarrow{w} - (\, 2\overrightarrow{v} + \overrightarrow{u}\,)$ 

 Lets do it in steps, first lets calculate $(\, 2\overrightarrow{v} + \overrightarrow{u}\,)$
 $$
\begin{align}
(\, 2\overrightarrow{v} + \overrightarrow{u}\,) &= \langle \, (2)\,2, \ (2)-3, \ (2)\,5 \, \rangle + \langle \, -1,\, 2,\, 3 \, \rangle\\
&=\langle \, 4, \ -6, \ 10 \, \rangle + \langle \, -1,\, 2,\, 3 \, \rangle\\
&= \langle \, 3,\, -4,\, 13 \, \rangle\\
\end{align}
$$
Then,  $\overrightarrow{u} + \overrightarrow{w}$
$$
\begin{align}
\overrightarrow{u} + \overrightarrow{w} &= 
\langle \, -1,\ 2,\ 3 \, \rangle + \langle \, 3,\, 5,\, -7 \,\rangle \\
&= \langle -2, 7, -4\rangle\\
\end{align}
$$
Finally 
$$
\begin{align}
\overrightarrow{u} + \overrightarrow{w} - (\, 2\overrightarrow{v} + \overrightarrow{u}\,) &= \langle \, 3,\, -4,\, 13 \, \rangle - \langle -2, 7, -4\rangle \\
&= \langle 5, -11, 17 \rangle\\
\end{align}
$$

## Question 3
- $\overrightarrow{u} \, \cdot \, \overrightarrow{v}$
$$
\begin{align}
\overrightarrow{u} \, \cdot \, \overrightarrow{v} &= \langle \, -1, 2, 3 \, \rangle \ \cdot \ \langle 2, -3, 5 \rangle\\
&= (\,(-1\cdot 2) \ + \ (2\cdot -3) \ + \ (3\cdot 5))\\
&= 7\\
\end{align}
$$

