$$
\begin{align}
E &= m \times i + 0 \times L & & \text{Total number or edges}\\
&= V - 1 & &\text{Edges is one less than total number of vertices }V\\
&=(i + L) - 1 & &\text{Substitute } V=i+L\\
m\times i + 0 \times L &= (i + L) - 1 & &\text{Set both expressions for } E \text{ to each other}\\
i (m-1) &= L - 1 & &\text{Arithmetic}\\
i &= \cfrac{(L-1)}{(m-1)} & &\text{Therefore,}
\end{align}
$$

$$
\begin{align}
E &= m \times i + 0 \times L &&\text{Total number of edges}\\
&= V - 1 &&\text{Edges is one less than the total number of vertices }V\\
&= (i + L) - 1 &&\text{Substitute } V = i + L\\
m \times i + 0 \times L &= (i + L) - 1 &&\text{Set both expressions for } E \text{ to each other}\\
i (m - 1) &= L - 1 &&\text{Arithmetic}\\
i &= \frac{L - 1}{m - 1} &&\text{Therefore,}
\end{align}
$$